---
layout: post
title:  "Basic properties of radicals"
date:   2019-12-13
author: Hidenori
---

# Proposition
1. $r(a) \supset a$.
1. $r(r(a))  = r(a)$.
1. $r(ab) = r(a \cap b) = r(a) \cap r(b)$.
1. $r(a) = (1) \iff a = (1)$.
1. $r(a + b) = r(r(a) + r(b))$.
1. if $p$ is prime, $r(p^n) = p$ for all $n > 0$.

# Solution
## 1
If $x \in a$, then $x^1 \in a$, so $x \in r(a)$.

## 2
By 1, $r(a) \subset r(r(a))$.
Let $x \in r(r(a))$.
Then $x^m \in r(a)$, and $(x^m)^n \in a$ for some $m, n \geq 1$.
Therefore, $x^{mn} \in a$, so $x \in r(a)$.

## 3
Since $ab \subset a \cap b$, $r(ab) \subset r(a \cap b)$.
Let $x \in r(a \cap b)$.
Then $x^m \in a \cap b$.
Thus $x^m \in a$ and $x^m \in b$, so $x^{2m} \in ab$.
Therefore, $x \in r(ab)$.

Let $x \in r(a \cap b)$.
Then $x^m \in a \cap b$, so $x^m \in a$ and $x^m \in b$.
Therefore, $x \in r(a)$ and $x \in r(b)$, so $x \in r(a) \cap r(b)$.
Let $x \in r(a) \cap r(b)$.
Then $x^m \in a$ and $x^n \in b$ for some $m, n \in \mathbb{Z}$.
Then $x^{m + n} \in a \cap b$, so $x \in r(a \cap b)$.
Thus $r(a \cap b) = r(a) \cap r(b)$.

## 4
If $r(a) = (1)$, then $1 \in r(a)$, so $1^m = 1 \in a$, so $a = (1)$.
If $a = (1)$, then $a \subset r(a)$, so $r(a) = 1$.


## 5
By 1, $a \subset r(a)$ and $b \subset r(b)$.
Then $a + b \subset r(a) + r(b)$, so $r(a + b) \subset r(r(a) + r(b))$.

Let $x \in r(r(a) + r(b))$.
Then $x^m \in r(a) + r(b)$ for some $m \in \mathbb{N}$.
Let $y \in r(a)$ and $z \in r(b)$ such that $x^m = y + z$.
Let $n, l \in \mathbb{N}$ be chosen such that $y^n \in a$ and $z^l \in b$.
Then $x^{n + l} = (y + z)^{n + l} = \sum_{i=0}^{n + l} \binom{n + l}{i} y^{i}z^{n + l - i} \in a + b$ because for each $i$, $i \geq n$ or $n + l - i \geq l$.
Therefore, $x \in r(a + b)$.
This implies $r(r(a) + r(b)) \subset r(a + b)$.

Thus $r(a + b) = r(r(a) + r(b))$.

## 6
By 1, $p \subset r(p)$.
Let $x \in r(p)$.
Then $x^m \in p$ for some $m \geq 1$.
Since $p$ is prime, $x \in p$.
Thus $p = r(p)$.

By 3, $r(p^n) = r(p) \cap r(p^{n - 1}) = p \cap r(p^{n - 1})$, so by induction, $r(p^n) = p$.


