---
layout: post
title:  "Zariski topology"
date:   2019-11-27
author: Hidenori
---

# Proposition
Let $A$ be a ring and let $X$ be the set of all prime ideals of $A$.
For each subset $E$ of $A$, let $V(E)$ denote the set of all prime ideals of $A$ which contain $E$.
Prove that

1. if $a$ is the ideal generated by $E$, then $V(E) = V(a) = V(r(a))$.
1. $V(0) = X, V(1) = \emptyset$.
1. If $$(E_i)_{i \in I}$$ is any family of subsets of $A$, then $$V(\cup_{i \in I} E_i) = \cap_{i \in I} V(E_i)$$.
1. $V(a \cap b) = V(ab) = V(a) \cup V(b)$ for any ideals $a, b$ of $A$.

# Solution

## 1
* Since $E \subset a$, $V(a) \subset V(E)$.
* Let $p \in V(E)$.
  Then $p$ is an ideal containing $E$.
  Since $a$ is the smallest ideal containing $E$, $a \subset p$.
  Therefore, $p \in V(a)$.

Therefore, $V(a) = V(E)$.

Since $a \subset r(a)$, $V(r(a)) \subset V(a)$.

Let $p \in V(a)$.
Then $p$ is a prime ideal containing $a$.
Let $x \in r(a)$.
If $x \in p$, we are done.

Suppose $x \notin p$.
Then $x^m \in a \subset p$ for some $m \geq 1$.
Then $x \cdot x^{m - 1} \in p$, so either $x$ or $x^{m - 1}$ is in $p$.
Since we assumed $x \notin p$, $x^{m - 1} \in p$.
However, by repeating this process, it will show that $x \in p$ after $m - 1$ steps.
Therefore, $x$ must be in $p$.

This means $r(a) \subset p$, so $p \in V(r(a))$.
Therefore, $V(r(a)) = V(a)$.

## 2
Since every prime ideal contains $0$, $V(0) = X$.
Since every prime ideal is a proper ideal, no prime ideal contains $1$.
Thus $V(1) = \emptyset$.

## 3

$$
\begin{align*}
  p \in V(\cup_{i \in I} E_i)
    &\iff \forall i \in I, E_i \subset p \\
    &\iff \forall i \in I, p \in V(E_i) \\
    &\iff p \in \cap_{i \in I} V(E_i).
\end{align*}
$$

## 4
Since $ab \subset a$ and $ab \subset b$, $ab \subset a \cap b$.
Therefore, $V(a \cap b) \subset V(ab)$.

Let $p \in V(ab)$.
Then $ab \subset p$.
Let $x \in a \cap b$.
Then $x^2 \in ab \subset p$, so $x \in p$.
Therefore, $a \cap b \subset p$, so $p \in V(a \cap b)$.

This shows $V(ab) = V(a \cap b)$.

Since $a \cap b \subset a$ and $a \cap b \subset b$, $V(a) \subset V(a \cap b)$ and $V(b) \subset V(a \cap b)$.
Thus, $V(a) \cup V(b) \subset V(a \cap b)$.

Let $p \in V(a \cap b)$.
If $a \subset p$, then $p \in V(a)$.
Suppose otherwise.
Let $x \in b$ and $y \in a \setminus p$.
Then $xy \in a \cap b \subset p$.
Since $p$ is prime and $y \notin p$, $x \in p$.
Therefore, $b \subset p$, so $p \in V(b)$.

Thus we have $p \in V(a) \cup V(b)$, so we have $V(a) \cup V(b) = V(a \cap b)$.

