---
layout: post
title:  "A basic property of a bimodule(WIP)"
date:   2019-11-30
author: Hidenori
---

# Proposition
Let $A, B$ be rings, let $M$ be an $A$-module, $P$ a $B$-module and $N$ an $(A, B)$-bimodule.
Then $M \otimes_A N$ is naturally a $B$-module, $N \otimes_B P$ an $A$-module, and we have

$$
\begin{align*}
  (M \otimes_A N) \otimes_B P \simeq M \oplus (N \oplus_B P).
\end{align*}
$$

# Solution
Let $z \in P$ be given.
Let $f_z:M \times N \rightarrow M \otimes_A (N \otimes_B P)$ be defined such that $f_z(x, y) = x \otimes (y \otimes z)$.
We claim that $f_z$ is $A$-bilinear.
For any $a \in A$ and $x, x' \in M$,

$$
\begin{align*}
  f_z(ax + x', y)
    &= (ax + x') \otimes (y \otimes z) \\
    &= ax \otimes (y \otimes z) + x' \otimes (y \otimes z) \\
    &= a(x \otimes (y \otimes z)) + x' \otimes (y \otimes z) \\
    &= af_z(x, y) + f_z(x', y).
\end{align*}
$$

Similarly, $f_z(x, ay + y') = af_z(x, y) + f_z(x, y')$ for any $a \in A$ and $y, y' \in N$.

Therefore, $f_z$ is $A$-bilinear.
By Proposition 2.12 [Atiyah], there must exist an $A$-linear mapping $f_z':M \otimes_A N \rightarrow (M \otimes_A (N \otimes_B P))$ such that $f_z(x, y) = f_z'(x \otimes y)$.
Moreover, $f_z'$ is $B$-linear because

1. $$
   \begin{align*}
   f_z'(x \otimes y + x' \otimes y) = f_z'(x \otimes y) + f(x' \otimes y)
   \end{align*}
   $$
1. $$
   \begin{align*}
     f_z'(b(x \otimes y))
       &= f_z'(x \otimes by) \\
       &= x \otimes (by \otimes z) \\
       &= x \otimes (b(y \otimes z)) \\
       &= b(x \otimes (y \otimes z)) \\
       &= bf_z'(x \otimes y).
   \end{align*}
   $$

The argument above works for any $z \in P$.

Now, we will define $f: (M \otimes_A N) \times B \rightarrow M \otimes_A (N \otimes_B P)$ such that $f(x \otimes y, z) = f_z'(x \otimes y)$.
We claim that $f$ is $B$-bilinear.

For any $b \in B$, $x \otimes y, x' \otimes y' \in M \otimes_A N$,

$$
\begin{align*}
  f(b(x \otimes y) + (x' \otimes y'), z)
    &= f_z'(b(x \otimes y) + (x' \otimes y')) \\
    &= bf_z'(x \otimes y) + f_z'(x' \otimes y') \\
    &= bf(x \otimes y, z) + f(x' \otimes y', z).
\end{align*}
$$

because $f_z'$ is $B$-linear as shown above.

TODO
