---
layout: post
title:  "Bilinear functions and their limits and derivatives"
date:   2019-12-25
author: Hidenori
---

# Proposition
A function $f: \mathbb{R}^n \times \mathbb{R}^m \rightarrow \mathbb{R}^p$ is bilinear if for $x, x_1, x_2 \in \mathbb{R}^n$, $y, y_1, y_2 \in \mathbb{R}^m$, and $a \in \mathbb{R}$ we have

$$
\begin{align*}
  f(ax, y) &= af(x, y) = f(x, ay), \\
  f(x_1 + x_2, y) &= f(x_1, y) + f(x_2, y), \\
  f(x, y_1 + y_2) &= f(x, y_1) + f(x, y_2).
\end{align*}
$$

1. Prove that if $f$ is bilinear, then
   $$
   \begin{align*}
     \lim\limits_{(h, k) \rightarrow 0} \frac{\abs{f(h, k)}}{\abs{(h, k)}} = 0.
   \end{align*}
   $$
1. Prove that $Df(a, b)(x, y) = f(a, y) + f(x, b)$.
1. Show that the formula for $Dp(a, b)$ in Theorem 2-3 is a special case of (b).

# Solution
## 1
Let $(h, k) = ((h_1, \cdots, h_n), (k_1, \cdots, k_m)) \in \mathbb{R}^n \times \mathbb{R}^m$ be given.

Let $u_i$'s and $v_j$'s denote the standard unit vectors in $\mathbb{R}^n$ and $\mathbb{R}^m$, respectively.

$$
\begin{align*}
  \abs{f(h, k)}
    &= \abs{\sum_{i=1}^n \sum_{j=1}^m f(h_iu_i, k_jv_j)} \\
    &\leq \abs{\sum_{i=1}^n \sum_{j=1}^m h_ik_jf(u_i, v_j)} \\
    &\leq \sum_{i=1}^n \sum_{j=1}^m \abs{h_ik_jf(u_i, v_j)} \\
    &= \sum_{i=1}^n \sum_{j=1}^m \abs{h_ik_j}\abs{f(u_i, v_j)}.
\end{align*}
$$

Let $M = \max\\{ \abs{f(u_i, v_j)} \\}$.

$$
\begin{align*}
  \sum_{i=1}^n \sum_{j=1}^m \abs{h_ik_j}\abs{f(u_i, v_j)}
    &\leq M \sum_{i=1}^n \sum_{j=1}^m \abs{h_ik_j}.
\end{align*}
$$

For each $i$ and $j$, $\abs{h_ik_j} \leq \max\\{\abs{h_i}^2, \abs{k_j}^2\\} \leq \abs{h_i}^2 + \abs{k_j}^2$.

$$
\begin{align*}
  \sum_{i=1}^n \sum_{j=1}^m \abs{h_ik_j}
    &\leq \sum_{i=1}^n \sum_{j=1}^m \abs{h_i}^2 + \abs{k_j}^2 \\
    &= m \sum_{i=1}^n \abs{h_i}^2 + n \sum_{j=1}^m \abs{k_j}^2 \\
    &< (m + n) \sum_{i=1}^n \abs{h_i}^2 + (m + n) \sum_{j=1}^m \abs{k_j}^2 \\
    &= (m + n) (\sum_{i=1}^n \abs{h_i}^2 + \sum_{j=1}^m \abs{k_j}^2) \\
    &= (m + n) \abs{(h, k)}^2.
\end{align*}
$$

By putting these together, we get $\abs{f(h, k)} < M(m + n)\abs{(h, k)}^2$ where $M(m + n)$ does not depend on the choice of $h, k$.

Therefore,

$$
\begin{align*}
  \lim\limits_{(h, k) \rightarrow 0} \frac{\abs{f(h, k)}}{\abs{(h, k)}}
    &\leq \lim\limits_{(h, k) \rightarrow 0} \frac{M(m + n)\abs{(h, k)}^2}{\abs{(h, k)}} \\
    &= \lim\limits_{(h, k) \rightarrow 0} M(m + n)\abs{(h, k)} \\
    &= 0.
\end{align*}
$$

## 2

Let $(a, b) \in \mathbb{R}^n \times \mathbb{R}^m$.

Let $A: \mathbb{R}^n \times \mathbb{R}^m \rightarrow \mathbb{R}^p$ be defined such that $A(x, y) = f(x, b) + f(a, y)$.
Then $A$ is linear since $\forall (x_1, y_1), (x_2, y_2) \in \mathbb{R}^n \times \mathbb{R}^m, \forall t \in \mathbb{R},$

$$
\begin{align*}
 A(c(x_1, y_1) + (x_2, y_2))
  &= A((cx_1 + x_2, cy_1 + y_2)) \\
  &= f(cx_1 + x_2, b) + f(a, cy_1 + y_2) \\
  &= cf(x_1, b) + f(x_2, b) + cf(a, y_1) + f(a, y_2) \\
  &= c(f(x_1, b) + f(a, y_1)) + f(x_2, b) + f(a, y_2) \\
  &= cA(x_1, y_1) + A(x_2, y_2).
\end{align*}
$$

$$
\begin{align*}
  \lim\limits_{(h, k) \rightarrow 0} \frac{\abs{f((a, b) + (h, k)) - f(a, b) - A(h, k)}}{\abs{(h, k)}}
    &= \lim\limits_{(h, k) \rightarrow 0} \frac{\abs{f(a, b) + f(h, b) + f(a, k) + f(h, k) - f(a, b) - A(h, k)}}{\abs{(h, k)}} \\
    &= \lim\limits_{(h, k) \rightarrow 0} \frac{\abs{f(h, b) + f(a, k) + f(h, k) - A(h, k)}}{\abs{(h, k)}} \\
    &= \lim\limits_{(h, k) \rightarrow 0} \frac{\abs{f(h, b) + f(a, k) + f(h, k) - f(h, b) - f(a, k)}}{\abs{(h, k)}} \\
    &= \lim\limits_{(h, k) \rightarrow 0} \frac{\abs{f(h, k)}}{\abs{(h, k)}} \\
    &= 0.
\end{align*}
$$

Therefore, $f$ is differentiable at $(a, b)$ and $Df(a, b)(x, y) = f(x, b) + f(a, y)$.

## 3
Let $s: \mathbb{R}^2 \rightarrow \mathbb{R}$ be defined such that $s(x, y) = xy$.

* $as(x, y) = a(xy) = (ax)y = s(ax, y)$.
* $as(x, y) = a(xy) = x(ay) = s(x, ay)$.
* $s(x_1 + x_2, y) = (x_1 + x_2)y = x_1y + x_2y = s(x_1, y) + s(x_2, y)$.
* $s(x, y_1 + y_2) = x(y_1 + y_2) = xy_1 + xy_2 = s(x, y_1) + s(x, y_2)$.

Therefore, $s$ is bilinear.
From (b), we know that $Ds(a, b)(x, y) = s(a, y) + s(x, b) = ay + xb$.
