---
layout: post
title:  "Basis and tensor algebra"
date:   2019-11-23
author: Hidenori
---

# Proposition
Let $e_1, \cdots, e_n$ be the usual basis of $\mathbb{R}^n$ and let $\phi_1, \cdots, \phi_n$ be the dual basis.
1. Show that $\phi_{i_1} \wedge \cdots \wedge \phi_{i_k}(e_{i_1}, \cdots, e_{i_k}) = 1$.
   What would the right side be if the factor $(k + l)!/k!/l!$ did not appear in the definition of $\wedge$?
1. TODO

# Solution
## 1

First, we claim that $\phi_{i_1} \wedge \cdots \wedge \phi_{i_k} = k! \Alt(\phi_{i_1} \otimes \cdots \otimes \phi_{i_k})$ for any $1 \leq k \leq n$.
If $k = 1$, then this is obvious.
Suppose we showed this for some $1 \leq k \leq n - 1$.

$$
\begin{align*}
  (\phi_{i_1} \wedge \cdots \wedge \phi_{i_k}) \wedge \phi_{i_{k + 1}}
    &= \frac{(k + 1)!}{k!1!}\Alt((\phi_{i_1} \wedge \cdots \wedge \phi_{i_k}) \otimes \phi_{i_{k + 1}}) \\
    &= (k + 1)\Alt((\phi_{i_1} \wedge \cdots \wedge \phi_{i_k}) \otimes \phi_{i_{k + 1}}) \\
    &= (k + 1)\Alt(k!\Alt(\phi_{i_1} \otimes \cdots \otimes \phi_{i_k}) \otimes \phi_{i_{k + 1}}) \\
    &= (k + 1)!\Alt(\Alt(\phi_{i_1} \otimes \cdots \otimes \phi_{i_k}) \otimes \phi_{i_{k + 1}}) \\
    &= (k + 1)!\Alt(\phi_{i_1} \otimes \cdots \otimes \phi_{i_k} \otimes \phi_{i_{k + 1}}).
\end{align*}
$$

Therefore, the claim is true for any $k$.

Let $k, i_1, \cdots, i_k$ be given.

$$
\begin{align*}
  (\phi_{i_1} \wedge \cdots \wedge \phi_{i_k})(e_{i_1}, \cdots, e_{i_k})
    &= k!\Alt(\phi_{i_1} \otimes \cdots \otimes \phi_{i_k})(e_{i_1}, \cdots, e_{i_k}) \\ 
    &= \frac{k!}{k!}\sum_{\sigma \in S_k} \sgn(\sigma) (\phi_{i_1} \otimes \cdots \otimes \phi_{i_k})(e_{i_{\sigma_1}}, \cdots, e_{i_{\sigma_k}}) \\ 
    &= (\phi_{i_1} \otimes \cdots \otimes \phi_{i_k})(e_{i_{1}}, \cdots, e_{i_{k}}) \\ 
    &= 1.
\end{align*}
$$

Suppose that the factor $(k + 1)!/k!l!$ does not appear in the definition of $\wedge$.
Then $\phi_{i_1} \wedge \cdots \wedge \phi_{i_k} = \Alt(\phi_{i_1} \otimes \cdots \otimes \phi_{i_k})$.
This can be shown by induction because 

$$
\begin{align*}
  (\phi_{i_1} \wedge \cdots \wedge \phi_{i_k}) \wedge \phi_{i_{k + 1}}
    &= \Alt((\phi_{i_1} \wedge \cdots \wedge \phi_{i_k}) \otimes \phi_{i_{k + 1}}) \\
    &= \Alt(\Alt(\phi_{i_1} \otimes \cdots \otimes \phi_{i_k}) \otimes \phi_{i_{k + 1}}) \\
    &= \Alt(\phi_{i_1} \otimes \cdots \otimes \phi_{i_{k + 1}}).
\end{align*}
$$

Let $k, i_1, \cdots, i_k$ be given.

$$
\begin{align*}
  (\phi_{i_1} \wedge \cdots \wedge \phi_{i_k})(e_{i_1}, \cdots, e_{i_k})
    &= \Alt(\phi_{i_1} \otimes \cdots \otimes \phi_{i_k})(e_{i_1}, \cdots, e_{i_k}) \\ 
    &= \frac{1}{k!}\sum_{\sigma \in S_k} \sgn(\sigma) (\phi_{i_1} \otimes \cdots \otimes \phi_{i_k})(e_{i_{\sigma_1}}, \cdots, e_{i_{\sigma_k}}) \\ 
    &= \frac{1}{k!}(\phi_{i_1} \otimes \cdots \otimes \phi_{i_k})(e_{i_{1}}, \cdots, e_{i_{k}}) \\ 
    &= \frac{1}{k!}.
\end{align*}
$$

## 2
TODO
